src/sep/PtsTo2.v
@@ -1,0 +1,229 @@
+Require Import DepList List.
+Require Import Expr SepExpr SymEval.
+Require Import Memory SepIL SymIL SepTac.
+
+Module BedrockPtsToEvaluator (P : EvaluatorPluginType BedrockHeap SepIL.ST).
+  Module Import SEP := P.SEP.
+
+  Definition pcIndex : nat := 0.
+  Definition stateIndex : nat := 1.
+  Definition pcT := tvType pcIndex.
+  Definition stT := tvType stateIndex.
+  
+  Definition wordIndex := 0.
+  Definition ptrIndex := 0.
+
+  Section parametric.
+    Variable types' : list type.
+    Definition types := bedrock_types ++ types'.
+  
+    Definition ptsto32_ssig : ssignature types pcT stT.
+    refine (
+      {| SepExpr.SDomain := tvType ptrIndex :: tvType wordIndex :: nil
+       ; SepExpr.SDenotation := _
+       |}).
+    refine (ptsto32 _).
+    Defined.
+
+    Variable funcs : functions types.
+
+    (** TODO: maybe this should be like unification? 
+     ** - in that case the substitution is an effect and needs to be
+     **   threaded through the computation (monadically?)
+     **)
+    Definition expr_equal (hyps : list (expr types)) (tv : tvar) (a b : expr types) : bool :=
+      match seq_dec a b with
+        | Some _ => true
+        | None => false
+      end.
+    Theorem expr_equal_correct : 
+      forall (hyps : list (expr types)) (tv : tvar) (a b : expr types),
+        expr_equal hyps tv a b = true ->
+        forall uvars vars,
+          AllProvable funcs uvars vars hyps ->
+          match exprD funcs uvars vars a tv , exprD funcs uvars vars b tv with 
+            | Some l , Some r => l = r
+            | _ , _ => True
+          end.
+    Proof.
+      unfold expr_equal. intros. destruct (seq_dec a b); subst.
+      destruct (exprD funcs uvars vars0 b tv); auto.
+      congruence.
+    Qed.
+
+  Definition sym_read_word_ptsto32 (hyps args : list (expr types)) (p : expr types) 
+    : option (expr types) :=
+    match args with
+      | p' :: v' :: nil => 
+        if expr_equal hyps (tvType ptrIndex) p p' then Some v' else None
+      | _ => None
+    end.
+  Definition sym_write_word_ptsto32 (hyps args : list (expr types)) (p v : expr types)
+    : option (list (expr types)) :=
+    match args with
+      | p' :: v' :: nil =>
+        if expr_equal hyps (tvType ptrIndex) p p' then Some (p :: v :: nil) else None
+      | _ => None
+    end.
+
+  Ltac expose :=
+    repeat (unfold wordIndex, ptrIndex in *; 
+            match goal with 
+              | [ H : match applyD _ _ ?A _ _ with
+                        | Some _ => _ 
+                        | None => False 
+                      end |- _ ] =>
+              destruct A; simpl in H; try (exfalso; assumption)
+              | [ H : context [ match exprD ?A ?B ?C ?D ?E with
+                          | None => _
+                          | Some _ => _
+                        end ] |- _ ] =>
+              revert H; case_eq (exprD A B C D E); simpl; intros; 
+                try (exfalso; assumption)
+              | [ H : context [ match expr_equal ?A ?B ?C ?D with
+                                  | true => _
+                                  | false => _
+                                end ] |- _ ] =>
+                revert H; case_eq (expr_equal A B C D); intros; 
+                  try (exfalso; congruence)
+              | [ H : expr_equal ?A ?B ?C ?D = true 
+                , H' : AllProvable _ _ _ ?A |- _ ] =>
+                generalize (@expr_equal_correct _ _ _ _ H _ _ H'); clear H; intros
+              | [ H : Some _ = Some _ |- _ ] =>
+                inversion H; clear H; subst
+              | [ H : exprD _ _ _ _ _ = Some _ |- _ ] =>
+                rewrite H in *
+            end; simpl in * ).
+
+  Lemma sym_read_ptsto32_correct : forall args uvars vars cs hyps pe p ve m stn,
+    sym_read_word_ptsto32 hyps args pe = Some ve ->
+    AllProvable funcs uvars vars hyps ->
+    exprD funcs uvars vars pe (tvType ptrIndex) = Some p ->
+    match 
+      applyD (exprD funcs uvars vars) (SDomain ptsto32_ssig) args _ (SDenotation ptsto32_ssig)
+      with
+      | None => False
+      | Some p => ST.satisfies cs p stn m
+    end ->
+    match exprD funcs uvars vars ve (tvType wordIndex) with
+      | Some v =>
+        ST.HT.smem_get_word (IL.implode stn) p m = Some v
+      | _ => False
+    end.
+  Proof.
+    simpl; intros.
+    unfold sym_read_word_ptsto32 in H.
+    repeat (destruct args; try congruence).
+    revert H.
+    case_eq (expr_equal hyps (tvType ptrIndex) pe e); try congruence.
+    intros.
+    inversion H3; clear H3; subst.
+    eapply expr_equal_correct in H; eauto.
+    simpl applyD in H2.
+    expose; try congruence.
+    unfold ST.satisfies in H6. PropXTac.propxFo. 
+  Qed.
+
+  Lemma sym_write_word_ptsto32_correct : forall args uvars vars cs hyps pe p ve v m stn args',
+    sym_write_word_ptsto32 hyps args pe ve = Some args' ->
+    AllProvable funcs uvars vars hyps ->
+    exprD funcs uvars vars pe (tvType ptrIndex) = Some p ->
+    exprD funcs uvars vars ve (tvType wordIndex) = Some v ->
+    match
+      applyD (@exprD _ funcs uvars vars) (SDomain ptsto32_ssig) args _ (SDenotation ptsto32_ssig)
+      with
+      | None => False
+      | Some p => ST.satisfies cs p stn m
+    end ->
+    match 
+      applyD (@exprD _ funcs uvars vars) (SDomain ptsto32_ssig) args' _ (SDenotation ptsto32_ssig)
+      with
+      | None => False
+      | Some pr => 
+        match ST.HT.smem_set_word (IL.explode stn) p v m with
+          | None => False
+          | Some sm' => ST.satisfies cs pr stn sm'
+        end
+    end.
+  Proof.
+    simpl; intros; expose; try congruence.
+
+    unfold ST.satisfies in *. PropXTac.propxFo. 
+    case_eq (smem_set_word (IL.explode stn) t v m).
+    intros. unfold ptsto32. PropXTac.propxFo.
+    eapply smem_set_get_word_eq; eauto.
+    eapply IL.implode_explode.
+    eapply smem_set_get_valid_word; eauto.
+  Qed.  
+
+  Definition SymEval_ptsto32 : @P.SymEval types stT pcT
+    (tvType ptrIndex) (tvType wordIndex)
+    SepTac.smem_read
+    SepTac.smem_write
+    funcs ptsto32_ssig.
+  eapply P.Build_SymEval.
+  eapply sym_read_ptsto32_correct.
+  eapply sym_write_word_ptsto32_correct.
+  Defined.  
+
+  End parametric.
+
+End BedrockPtsToEvaluator.
+
+Module DEMO := BedrockPtsToEvaluator SymIL.PLUGIN.
+
+Import BedrockEvaluator.
+
+Record mem_evaluator : Type :=
+{ READER : _ 
+; WRITER : _
+; CORRECTNESS : BedrockEvaluator.Correctness READER WRITER
+}.
+
+(** TODO: I need to find some way to build this using tactics! **)
+Definition ptsto_evaluator : mem_evaluator.
+refine (
+  {| READER := fun typs hyps p s =>
+    match FM.find 0 (impures s) with
+      | None => None
+      | Some argss =>
+        @fold_args unit (fun _ => unit) (bedrock_types ++ typs) (expr (bedrock_types ++ typs)) 
+          (fun _ _ args =>
+            match args with
+              | p' :: v' :: nil => 
+                if DEMO.expr_equal _ hyps (tvType 0) p p' then Some v' else None
+              | _ => None
+            end)
+          tt tt argss
+    end
+   ; WRITER := fun typs hyps p v s => 
+     match FM.find 0 (impures s) with
+      | None => None
+      | Some argss =>
+        let res :=
+          @fold_args_update unit (fun _ => unit) (bedrock_types ++ typs)
+            (fun _ _ args =>
+              match args with
+                | p' :: v' :: nil => 
+                  if DEMO.expr_equal _ hyps (tvType 0) p p' then Some (p' :: v :: nil) else None
+                | _ => None
+              end)
+            tt tt argss
+        in
+        match res with
+          | None => None
+          | Some res =>
+            Some {| impures := FM.add 0 res (impures s) ; pures := pures s ; other := other s |}
+        end
+    end
+   ; CORRECTNESS := 
+     {| TypeImage := nil
+      ; FuncImage := fun _ => nil
+      ; PredImage := fun t => (0, DEMO.ptsto32_ssig t) :: nil
+      ; ReadCorrect := _
+      ; WriteCorrect := _
+      |}
+   |}); unfold READER, WRITER.
+admit.
+admit.
+Defined.
